wip

Cfg.dfy
@@ -49,67 +49,72 @@ module BoogieCfg {
     post: Predicate<A>, 
     cover: set<BlockId>) : Predicate<A>
     requires g.successors.Keys <= g.blocks.Keys //not being in the domain of the successor relation is the same as not having any successors
-    requires IsAcyclicSeq(g.successors, ns, cover)
+    requires |ns| >= 1
     decreases cover, 1, ns
-  { s =>
-      if |ns| == 0 then Some(true)
+  {   //this definition allows one to deduce that WpCfgConjunction and WpCfg coincide for singleton sequences (instead of just being pointwise equal)
+      if |ns| == 1 then WpCfg(a, g, ns[0], post, cover) 
       else 
-        var res1 :- WpCfg(a, g, ns[0], post, cover)(s);
-        var res2 :- WpCfgConjunction(a, g, ns[1..], post, cover)(s);
-        Some(res1 && res2)
+        s => 
+          var res1 :- WpCfg(a, g, ns[0], post, cover)(s);
+          var res2 :- WpCfgConjunction(a, g, ns[1..], post, cover)(s);
+          Some(res1 && res2)
   }
 
   function WpCfg<A(!new)>(a: absval_interp<A>, g: Cfg, n: BlockId, post: Predicate<A>, cover: set<BlockId>) : Predicate<A>
     requires g.successors.Keys <= g.blocks.Keys //not being in the domain of the successor relation is the same as not having any successors
-    requires IsAcyclic(g.successors, n, cover)
     decreases cover, 0
   {
-    if !(n in g.blocks.Keys) then
-      post
-    else 
-      var successors := if n in g.successors.Keys then g.successors[n] else [];
-      if |successors| == 0 then 
-        WpShallowSimpleCmd(a, g.blocks[n], post)
+    if IsAcyclic(g.successors, n, cover) then
+      if n !in g.blocks.Keys then
+        post
       else 
-        WpShallowSimpleCmd(a, g.blocks[n], WpCfgConjunction(a, g, successors, post, cover - {n}))
+        var successors := if n in g.successors.Keys then g.successors[n] else [];
+        if |successors| == 0 then 
+          WpShallowSimpleCmd(a, g.blocks[n], post)
+        else 
+          WpShallowSimpleCmd(a, g.blocks[n], WpCfgConjunction(a, g, successors, post, cover - {n}))
+    else 
+      s => None
   }
-
 
   lemma WpCfgConjunctionPointwise<A(!new)>(a: absval_interp<A>, g: Cfg, ns: seq<BlockId>, post1: Predicate<A>, post2: Predicate<A>, cover: set<BlockId>, s: state<A>) 
     requires g.successors.Keys <= g.blocks.Keys //not being in the domain of the successor relation is the same as not having any successors
-    requires IsAcyclicSeq(g.successors, ns, cover)
+    //requires IsAcyclicSeq(g.successors, ns, cover)
     requires (forall s :: post1(s) == post2(s))
+    requires |ns| >= 1
     ensures WpCfgConjunction(a, g, ns, post1, cover)(s) == WpCfgConjunction(a, g, ns, post2, cover)(s)
     decreases cover, 1, ns
   {
-    if |ns| > 0 {
-      WpCfgPointwise(a, g, ns[0], post1, post2, cover, s);
+    WpCfgPointwise(a, g, ns[0], post1, post2, cover, s);
+    if |ns| > 1 {
       WpCfgConjunctionPointwise(a, g, ns[1..], post1, post2, cover, s);
     }
   }
 
   lemma WpCfgPointwise<A(!new)>(a: absval_interp<A>, g: Cfg, n: BlockId, post1: Predicate<A>, post2: Predicate<A>, cover: set<BlockId>, s: state<A>)
     requires g.successors.Keys <= g.blocks.Keys //not being in the domain of the successor relation is the same as not having any successors
-    requires IsAcyclic(g.successors, n, cover)
+    //requires IsAcyclic(g.successors, n, cover)
     requires (forall s :: post1(s) == post2(s))
     ensures WpCfg(a, g, n, post1, cover)(s) == WpCfg(a, g, n, post2, cover)(s)
     decreases cover, 0
   {
-    if n in g.blocks.Keys {
-      var block := g.blocks[n];
-      var successors := if n in g.successors.Keys then g.successors[n] else [];
-      if |successors| == 0  {
-        WpShallowSimpleCmdPointwise(a, block, post1, post2, s);
-      } else {
-        var successorPost1 := WpCfgConjunction(a, g, successors, post1, cover - {n});
-        var successorPost2 := WpCfgConjunction(a, g, successors, post2, cover - {n});
-        
-        forall s' | true
-          ensures successorPost1(s') == successorPost2(s')
-        {
-          WpCfgConjunctionPointwise(a, g, successors, post1, post2, cover - {n}, s');
+    if IsAcyclic(g.successors, n, cover) {
+      if n in g.blocks.Keys {
+        var block := g.blocks[n];
+        var successors := if n in g.successors.Keys then g.successors[n] else [];
+        if |successors| == 0  {
+          WpShallowSimpleCmdPointwise(a, block, post1, post2, s);
+        } else {
+          var successorPost1 := WpCfgConjunction(a, g, successors, post1, cover - {n});
+          var successorPost2 := WpCfgConjunction(a, g, successors, post2, cover - {n});
+          
+          forall s' | true
+            ensures successorPost1(s') == successorPost2(s')
+          {
+            WpCfgConjunctionPointwise(a, g, successors, post1, post2, cover - {n}, s');
+          }
+          WpShallowSimpleCmdPointwise(a, block, successorPost1, successorPost2, s);
         }
-        WpShallowSimpleCmdPointwise(a, block, successorPost1, successorPost2, s);
       }
     }
   }
@@ -130,94 +135,6 @@ module BoogieCfg {
            var nsPre := WpCfgConjunction(a, g, ns, post, cover)(s);
            ImpliesOpt(nsPre, nPre)
   /** TODO proof */
- 
-  /*============================Operational semantics========================*/
-
-  least predicate CfgRed<A(!new)>(a: absval_interp<A>, g: Cfg, n: BlockId, s: ExtState<A>, s': ExtState<A>)
-    requires g.blocks.Keys == g.successors.Keys
-  {
-    if n in g.blocks.Keys then
-      var blocks := g.blocks[n];
-      var successors := g.successors[n];
-
-      if |successors| == 0 then
-        SimpleCmdOpSem(a, blocks, s, s')
-      else
-        assert successors[0] in successors; //required for non-emptiness constraint in next line to go through
-        var succ :| succ in successors;
-        (exists s'' :: SimpleCmdOpSem(a, blocks, s, s'') && CfgRed(a, g, succ, s'' , s'))
-    else 
-      false
-  }
-
-/*==========Correspondence Wp and Operational Semantics===========================*/
-
-  lemma WpSemToOpSem_SimpleCmd<A(!new)>(a: absval_interp<A>, scs: SimpleCmd, post: Predicate<A>, s: state<A>, s': ExtState<A>)
-    requires WpShallowSimpleCmd(a, scs, post)(s) == Some(true)
-    requires SimpleCmdOpSem(a, scs, NormalState(s), s')
-    ensures s' != FailureState
-    ensures forall ns' :: s' == NormalState(ns') ==> post(ns') == Some(true)
-  /** TODO proof */
- 
-  //Note that the following lemma is trivially satisfied if CfgRed is the empty relation
-  lemma WpSemToOpSem<A(!new)>(a: absval_interp<A>, g: Cfg, n: BlockId, post: Predicate<A>, cover: set<BlockId>, s: state<A>, s': ExtState<A>)
-    requires IsAcyclic(g.successors, n, cover)
-    requires g.successors.Keys == g.blocks.Keys
-    requires WpCfg(a, g, n, post, cover)(s) == Some(true)
-    requires CfgRed(a, g, n, NormalState(s), s')
-    requires CfgWf(g) && n in g.blocks.Keys
-    ensures s' != FailureState
-    ensures forall ns' :: s' == NormalState(ns') ==> post(ns') == Some(true)
-    decreases cover
-  {
-    var block := g.blocks[n];
-    var successors := g.successors[n];
-
-    if |successors| == 0 {
-      WpSemToOpSem_SimpleCmd(a, block, post, s, s');
-    } else {
-      assert WpShallowSimpleCmd(a, block, WpCfgConjunction(a, g, successors, post, cover - {n}))(s) == Some(true);
-
-      var succ, y :| succ in successors && SimpleCmdOpSem(a, block, NormalState(s), y) && CfgRed(a, g, succ, y , s');
-
-      WpSemToOpSem_SimpleCmd(a, block, WpCfgConjunction(a, g, successors, post, cover - {n}), s, y);
-
-      match y {
-        case MagicState => assume false; //TODO magic state stays magic
-        case NormalState(s'') => 
-        calc {
-          IsAcyclic(g.successors, n, cover);
-          ==>
-          IsAcyclicSeq(g.successors, successors, cover - {n});
-          ==> { IsAcyclicElem(g.successors, successors, succ, cover - {n}); }
-          IsAcyclic(g.successors, succ, cover - {n});
-        }
-        assert WpCfg(a, g, succ, post, cover - {n})(s'') == Some(true) by {
-          WpCfgConjunctionSingle(a, g, successors, succ, post, cover - {n}, s'');
-        }
-        
-        WpSemToOpSem(a, g, succ, post, cover - {n}, s'', s');
-      }
-    }
-  }
-
-  /** TODO OpSem to WP */
-  function CfgRedSet<A(!new)>(a: absval_interp<A>, g: Cfg, n: BlockId, y: ExtState<A>) : iset<ExtState<A>>
-    requires g.blocks.Keys == g.successors.Keys
-  {
-    iset y' | CfgRed(a, g, n, y, y')
-  }
-
-  lemma OpSemToWpSem<A(!new)>(a: absval_interp<A>, g: Cfg, n: BlockId, post: Predicate<A>, cover: set<BlockId>, s: state<A>)
-    requires IsAcyclic(g.successors, n, cover)
-    requires g.successors.Keys == g.blocks.Keys
-    requires !(FailureState in CfgRedSet(a, g, n, NormalState(s)))
-    requires CfgWf(g) && n in g.blocks.Keys
-    ensures var wpRes := WpCfg(a, g, n, s' => Some(NormalState(s') in CfgRedSet(a, g, n, NormalState(s))), cover)(s);
-            wpRes == Some(true) || wpRes == None
-    decreases cover
-  /** TODO: proof */
-
   /*======================Acyclicity lemmas ===================================*/
 
   lemma IsAcyclicElem(r: SuccessorRel, ns: seq<BlockId>, nSucc: BlockId, cover: set<BlockId>)
@@ -333,8 +250,7 @@ module BoogieCfg {
     exit1: BlockId, 
     post: Predicate<A>, 
     cover1: set<BlockId>, 
-    cover2: set<BlockId>, 
-    s: state<A>)
+    cover2: set<BlockId>)
 
   lemma WpCfgMerge<A(!new)>(
     a: absval_interp<A>, 
@@ -344,12 +260,10 @@ module BoogieCfg {
     exit1: BlockId, 
     post: Predicate<A>, 
     cover1: set<BlockId>, 
-    cover2: set<BlockId>, 
-    s: state<A>)
+    cover2: set<BlockId>)
     requires g1.successors.Keys <= g1.blocks.Keys
     requires g2.successors.Keys <= g2.blocks.Keys
-    requires exit1 in g1.blocks.Keys
-    requires exit1 !in g1.successors.Keys
+    requires exit1 in g1.blocks.Keys && exit1 !in g1.successors.Keys
     requires g1.blocks.Keys !! g2.blocks.Keys
     requires IsAcyclic(g1.successors, g1Entry, cover1)
     requires IsAcyclic(g2.successors, g2.entry, cover2)
@@ -363,61 +277,148 @@ module BoogieCfg {
         (forall i :: 0 <= i < |g1.successors[n1]| ==> (g1.successors[n1][i] in g1.successors.Keys || 
                                                          g1.successors[n1][i] == exit1))
 
-    requires g1Entry in g1.blocks.Keys
+    requires g1Entry in g1.successors.Keys || g1Entry == exit1
+    requires g2.entry != exit1
+
+    requires forall n1 :: n1 in g1.successors.Keys ==> g1.successors[n1] != []
 
     // successors in g2.successors are not recorded in g1.successors
     requires
       forall n2 :: n2 in g2.successors.Keys ==>   
-        (forall i :: 0 <= i < |g2.successors[n2]| ==> !(g2.successors[n2][i] in g1.successors.Keys))
+        (forall i :: 0 <= i < |g2.successors[n2]| ==> !(g2.successors[n2][i] in g1.successors.Keys + {exit1}))
     ensures 
       var successors' := (g1.successors[exit1 := [g2.entry]] + g2.successors);
       var mergedCfg := Cfg(g1Entry, g1.blocks + g2.blocks, successors');
-      WpCfg(a, g1, g1Entry, WpCfg(a, g2, g2.entry, post, cover2), cover1)(s) ==
-      WpCfg(a, mergedCfg, g1Entry, post, cover1+cover2+{exit1})(s)
-    /*{
-      assert g1Entry in g1.blocks.Keys;
-      assert g1.successors.Keys <= g1.blocks.Keys;
-
+      WpCfg(a, g1, g1Entry, WpCfg(a, g2, g2.entry, post, cover2), cover1) ==
+      WpCfg(a, mergedCfg, g1Entry, post, cover1+cover2+{exit1})
+    {
+      var cover3 := cover1+cover2+{exit1};
       var block := g1.blocks[g1Entry];
       var successors := if g1Entry in g1.successors.Keys then g1.successors[g1Entry] else [];
 
-      var successors' := (g1.successors + g2.successors)[exit1 := [g2.entry]];
+      var successors' := (g1.successors[exit1 := [g2.entry]] + g2.successors);
       var mergedCfg := Cfg(g1Entry, g1.blocks + g2.blocks, successors');
-      assume IsAcyclic(mergedCfg.successors, g1Entry, cover1+cover2);
+
+      calc {
+        WpCfg(a, g2, g2.entry, post, cover2);
+          { WpCfgLargerCover(a, g2, g2.entry, post, cover2, cover3); }
+        WpCfg(a, g2, g2.entry, post, cover3);
+          { IsAcyclicLargerCover(g2.successors, g2.entry, cover2, cover3);
+            WpCfgExtend(a, mergedCfg, g2, g1.successors[exit1 := [g2.entry]], g2.entry, post, cover3); }
+        WpCfg(a, mergedCfg, g2.entry, post, cover3);
+      }
 
       if |successors| == 0 {
         assert g1Entry == exit1;
+
         calc {
-          WpCfg(a, g1, g1Entry, WpCfg(a, g2, g2.entry, post, cover2), cover1)(s);
-          WpShallowSimpleCmd(a, block, WpCfg(a, g2, g2.entry, post, cover2))(s);
-          WpCfg(a, mergedCfg, g1Entry, WpCfg(a, mergedCfg, g2.entry, post, cover2), cover1)(s);
-          WpCfg(a, mergedCfg, g1Entry, post, cover1)(s);
+          WpCfg(a, mergedCfg, g1Entry, post, cover3);
+          WpShallowSimpleCmd(a, block, WpCfgConjunction(a, mergedCfg, [g2.entry], post, cover3 - {g1Entry}));
+          WpShallowSimpleCmd(a, block, WpCfg(a, mergedCfg, g2.entry, post, cover3 - {g1Entry})); 
+            { WpCfgLargerCover(a, mergedCfg, g2.entry, post, cover3 - {g1Entry}, cover3); }
+          WpShallowSimpleCmd(a, block, WpCfg(a, mergedCfg, g2.entry, post, cover3));
+            { assert WpCfg(a, mergedCfg, g2.entry, post, cover3) == WpCfg(a, g2, g2.entry, post, cover2); }
+          WpShallowSimpleCmd(a, block, WpCfg(a, g2, g2.entry, post, cover2));
+          WpCfg(a, g1, g1Entry, WpCfg(a, g2, g2.entry, post, cover2), cover1);
         }
       } else {
-        assume false;  
+        assert g1.blocks[g1Entry] == mergedCfg.blocks[g1Entry];
+        calc {
+          WpCfg(a, mergedCfg, g1Entry, post, cover3);
+          WpShallowSimpleCmd(a, block, WpCfgConjunction(a, mergedCfg, successors, post, cover3-{g1Entry}));
+            { assume false; }
+          WpShallowSimpleCmd(a, block, WpCfgConjunction(a, g1, successors, WpCfg(a, g2, g2.entry, post, cover2), cover1-{g1Entry}));
+          WpCfg(a, g1, g1Entry, WpCfg(a, g2, g2.entry, post, cover2), cover1);
+        }
       }
-    }*/
+    }
 
-
-  lemma WpCfgExtend<A(!new)>(
+  
+  lemma WpCfgConjunctionLargerCover<A(!new)>(
     a: absval_interp<A>, 
-    g1: Cfg,
-    g2: Cfg,
-    exit1: BlockId, 
+    g: Cfg,
+    ns: seq<BlockId>,
+    post: Predicate<A>, 
+    cover1: set<BlockId>, 
+    cover2: set<BlockId>)
+  requires g.successors.Keys <= g.blocks.Keys
+  requires |ns| >= 1
+  requires cover1 <= cover2
+  requires IsAcyclicSeq(g.successors, ns, cover1)
+  ensures WpCfgConjunction(a, g, ns, post, cover1) == WpCfgConjunction(a, g, ns, post, cover2)
+  decreases cover1, 1, ns
+  {
+    WpCfgLargerCover(a, g, ns[0], post, cover1, cover2);
+  }
+
+  lemma WpCfgLargerCover<A(!new)>(
+    a: absval_interp<A>, 
+    g: Cfg,
+    n: BlockId,
     post: Predicate<A>, 
     cover1: set<BlockId>, 
     cover2: set<BlockId>) 
-    requires g1.successors.Keys <= g1.blocks.Keys
-    requires g2.successors.Keys <= g2.blocks.Keys
-    requires IsAcyclic(g2.successors, g2.entry, cover2)
-    requires exit1 in g1.blocks.Keys
-    ensures 
-      var successors' := (g1.successors + g2.successors)[exit1 := [g2.entry]];
-      var mergedCfg := Cfg(g1.entry, g1.blocks + g2.blocks, successors');
-      assume IsAcyclic(mergedCfg.successors, g2.entry, cover1+cover2);
+  requires g.successors.Keys <= g.blocks.Keys
+  requires cover1 <= cover2
+  requires IsAcyclic(g.successors, n, cover1)
+  ensures WpCfg(a, g, n, post, cover1) == WpCfg(a, g, n, post, cover2)
+  decreases cover1, 0
+  {
+    IsAcyclicLargerCover(g.successors, n, cover1, cover2);
+    
+    var successors := if n in g.successors.Keys then g.successors[n] else [];
 
-      WpCfg(a, g2, g2.entry, post, cover2) ==
-      WpCfg(a, mergedCfg, g2.entry, post, cover1+cover2)
+    if |successors| > 0 {
+      WpCfgConjunctionLargerCover(a, g, successors, post, cover1-{n}, cover2-{n});
+    }
+  }
+
+  lemma WpCfgConjunctionExtend<A(!new)>(a: absval_interp<A>, cfgMerged: Cfg, cfg2: Cfg, r1: SuccessorRel, ns: seq<BlockId>, post: Predicate<A>, cover: set<BlockId>)
+    requires 
+      var r2 := cfg2.successors;
+      && |ns| >= 1
+      && cfgMerged.successors == r1 + r2
+      && r1.Keys !! r2.Keys
+      && (forall n :: n in cfg2.blocks.Keys ==> n in cfgMerged.blocks.Keys && cfgMerged.blocks[n] == cfg2.blocks[n])
+      && cfgMerged.successors.Keys <= cfgMerged.blocks.Keys
+      && cfg2.successors.Keys <= cfg2.blocks.Keys
+      && IsAcyclicSeq(r2, ns, cover)
+      && (forall n :: n in ns ==> n !in r1.Keys && (n !in r2.Keys ==> n !in cfgMerged.blocks.Keys))
+      && (forall n2 :: n2 in r2.Keys ==>   
+           (forall i :: 0 <= i < |r2[n2]| ==> r2[n2][i] in r2.Keys || r2[n2][i] !in cfgMerged.blocks.Keys))
+    ensures WpCfgConjunction(a, cfgMerged, ns, post, cover) == WpCfgConjunction(a, cfg2, ns, post, cover)
+    decreases cover, 1, ns
+  {
+    WpCfgExtend(a, cfgMerged, cfg2, r1, ns[0], post, cover);
+  }
+
+  lemma WpCfgExtend<A(!new)>(a: absval_interp<A>, cfgMerged: Cfg, cfg2: Cfg, r1: SuccessorRel, n2Entry: BlockId, post: Predicate<A>, cover: set<BlockId>)
+    requires 
+      var r2 := cfg2.successors;
+      && cfgMerged.successors == r1 + r2
+      && r1.Keys !! r2.Keys
+      && (forall n :: n in cfg2.blocks.Keys ==> n in cfgMerged.blocks.Keys && cfgMerged.blocks[n] == cfg2.blocks[n])
+      && cfgMerged.successors.Keys <= cfgMerged.blocks.Keys
+      && cfg2.successors.Keys <= cfg2.blocks.Keys
+      && IsAcyclic(r2, n2Entry, cover)
+      && n2Entry !in r1.Keys && (n2Entry !in r2.Keys ==> n2Entry !in cfgMerged.blocks.Keys)
+      && (forall n2 :: n2 in r2.Keys ==>   
+           (forall i :: 0 <= i < |r2[n2]| ==> r2[n2][i] in r2.Keys || r2[n2][i] !in cfgMerged.blocks.Keys))
+    ensures WpCfg(a, cfgMerged, n2Entry, post, cover) == WpCfg(a, cfg2, n2Entry, post, cover)
+    decreases cover, 0
+  {
+    var successors := if n2Entry in cfg2.successors.Keys then cfg2.successors[n2Entry] else [];
+    IsAcyclicExtend(r1, cfg2.successors, n2Entry, cover);
+    assert IsAcyclic(cfgMerged.successors, n2Entry, cover);
+
+    if n2Entry in cfg2.blocks.Keys {
+      var block := cfg2.blocks[n2Entry];
+      assert n2Entry in cfgMerged.blocks.Keys;
+      if |successors| > 0 {
+        WpCfgConjunctionExtend(a, cfgMerged, cfg2, r1, successors, post, cover - {n2Entry});
+      }
+    } 
+  }
 
   lemma IsAcyclicExtendSeq(r1: SuccessorRel, r2: SuccessorRel, ns: seq<BlockId>, cover: set<BlockId>)
     requires IsAcyclicSeq(r2, ns, cover)
